Definitional interpreter with stores and booleans

examples/definterp.v
@@ -9,6 +9,7 @@ Derive Signature NoConfusion NoConfusionHom for t.
 
 Inductive Ty : Set :=
 | unit : Ty
+| bool : Ty
 | arrow (t u : Ty) : Ty
 | ref : Ty -> Ty.
 
@@ -24,12 +25,16 @@ Inductive In {A} (x : A) : list A -> Type :=
 | here {xs} : x ∈ (x :: xs)
 | there {y xs} : x ∈ xs -> x ∈ (y :: xs)
 where " x ∈ s " := (In x s).
+Derive Signature NoConfusion for In.
 
 Arguments here {A x xs}.
 Arguments there {A x y xs} _.
 
 Inductive Expr : Ctx -> Ty -> Set :=
 | tt {Γ} : Expr Γ unit
+| true {Γ} : Expr Γ bool
+| false {Γ} : Expr Γ bool
+| ite {Γ t} : Expr Γ bool -> Expr Γ t -> Expr Γ t -> Expr Γ t
 | var {Γ} {t} : In t Γ -> Expr Γ t
 | abs {Γ} {t u} : Expr (t :: Γ) u -> Expr Γ (t ⇒ u)
 | app {Γ} {t u} : Expr Γ (t ⇒ u) -> Expr Γ t -> Expr Γ u
@@ -56,16 +61,18 @@ End MapAll.
 
 Definition StoreTy := list Ty.
 
-Inductive Val : StoreTy -> Ty -> Set :=
-| val_unit {Σ} : Val Σ unit
-| val_closure {Σ Γ t u} : Expr (t :: Γ) u -> All (Val Σ) Γ -> Val Σ (t ⇒ u)
-| val_loc {Σ t} : t ∈ Σ -> Val Σ (ref t).
+Inductive Val : Ty -> StoreTy -> Set :=
+| val_unit {Σ} : Val unit Σ
+| val_true {Σ} : Val bool Σ
+| val_false {Σ} : Val bool Σ
+| val_closure {Σ Γ t u} : Expr (t :: Γ) u -> All (fun t => Val t Σ) Γ -> Val (t ⇒ u) Σ
+| val_loc {Σ t} : t ∈ Σ -> Val (ref t) Σ.
 
 Derive Signature NoConfusion NoConfusionHom for Val.
 
-Definition Env (Γ : Ctx) (Σ : StoreTy) : Set := All (Val Σ) Γ.
+Definition Env (Γ : Ctx) (Σ : StoreTy) : Set := All (fun t => Val t Σ) Γ.
 
-Definition Store (Σ : StoreTy) := All (Val Σ) Σ.
+Definition Store (Σ : StoreTy) := All (fun t => Val t Σ) Σ.
 
 Equations lookup : forall {A P xs} {x : A}, All P xs -> x ∈ xs -> P x :=
   lookup (all_cons p _) here := p;
@@ -75,76 +82,204 @@ Equations update : forall {A P xs} {x : A}, All P xs -> x ∈ xs -> P x -> All P
   update (all_cons p ps) here        p' := all_cons p' ps;
   update (all_cons p ps) (there ins) p' := all_cons p (update ps ins p').
 
-Equations lookup_store {Σ t} : t ∈ Σ -> Store Σ -> Val Σ t :=
+Equations lookup_store {Σ t} : t ∈ Σ -> Store Σ -> Val t Σ :=
   lookup_store l σ := lookup σ l.
 
-Equations update_store {Σ t} : t ∈ Σ -> Val Σ t -> Store Σ -> Store Σ :=
+Equations update_store {Σ t} : t ∈ Σ -> Val t Σ -> Store Σ -> Store Σ :=
   update_store l v σ := update σ l v.
 Import Sigma_Notations.
 
-Definition store_incl (Σ Σ' : StoreTy) := &{ Σ'' : _ & Σ' = Σ ++ Σ'' }.
+Definition store_incl (Σ Σ' : StoreTy) := &{ Σ'' : _ & Σ' = Σ'' ++ Σ }.
 Infix "⊑" := store_incl (at level 10).
+
+Lemma app_assoc {A} (x y z : list A) : x ++ y ++ z = (x ++ y) ++ z.
+Proof. induction x; simpl; auto.
+       now rewrite IHx.
+Defined.
 
 Section StoreIncl.
   Context {Σ Σ' : StoreTy} (incl : Σ ⊑ Σ').
 
   Lemma pres_in t : t ∈ Σ -> t ∈ Σ'.
-  Proof. destruct incl. subst. induction 1. econstructor; auto.
-         red in incl. destruct incl. apply List.app_inv_head in pr2. subst.
-         constructor 2. simpl.
-         apply IHIn. now exists pr0.
+  Proof. destruct incl. subst. clear. induction pr1. intros. exact H.
+         intros H. specialize (IHpr1 H). constructor 2. apply IHpr1.
   Defined.
 
-  Equations(noind) weaken_val {t} (v : Val Σ t) : Val Σ' t :=
+  Equations(noind) weaken_val {t} (v : Val t Σ) : Val t Σ' :=
    weaken_val val_unit := val_unit;
+   weaken_val val_true := val_true;
+   weaken_val val_false := val_false;
    weaken_val (val_closure b e) := val_closure b (map_all (fun t v => weaken_val v) e);
    weaken_val (val_loc H) := val_loc (pres_in _ H).
 
   Definition weaken_env {Γ} (v : Env Γ Σ) : Env Γ Σ' :=
     map_all (@weaken_val) v.
 
+  Lemma refl_incl : Σ ⊑ Σ.
+  Proof. exists []. reflexivity. Defined.
+
   Lemma trans_incl {Σ''} (incl' : Σ' ⊑ Σ'') : Σ ⊑ Σ''.
   Proof.
     destruct incl as [? ->], incl' as [? ->].
-    exists (pr1 ++ pr0). now rewrite app_assoc.
-  Qed.
+    exists (pr0 ++ pr1). now rewrite app_assoc.
+  Defined.
+
+  Lemma store_ext_incl {t} : Σ ⊑ (t :: Σ).
+  Proof. now exists [t]. Defined.
 
 End StoreIncl.
 
 Infix "⊚" := trans_incl (at level 10).
 
-Equations M : forall (Γ : Ctx) (P : StoreTy -> Set) (Σ : StoreTy), Type :=
-  M Γ P Σ := forall (E : Env Σ Γ) (μ : Store Σ), option &{ Σ' : _ & Store Σ' * P Σ' * Σ ⊑ Σ'}.
+Equations M : forall (Γ : Ctx) (P : StoreTy -> Type) (Σ : StoreTy), Type :=
+  M Γ P Σ := forall (E : Env Γ Σ) (μ : Store Σ), option &{ Σ' : _ & &{ _ : Store Σ' & &{ _ : P Σ' & Σ ⊑ Σ'}}}.
 
 Require Import Utf8.
+Notation "( x , .. , y , z )" := (sigmaI _ x .. (sigmaI _ y z) ..) : core_scope.
 
-Equations bind {Σ Γ} {P Q : StoreTy -> Type} (f : M Γ P Σ) (g : ∀ {Σ'}, P Σ' -> M Γ Q Σ') → M Γ Q Σ :=
-  bind f g E μ := match m E μ with
-                  | None => None
-                  | Some (x => f x γ
-              end.
+Equations bind {Σ Γ} {P Q : StoreTy -> Type} (f : M Γ P Σ) (g : ∀ {Σ'}, P Σ' -> M Γ Q Σ') : M Γ Q Σ :=
+  bind f g E μ with f E μ :=
+    { | None := None;
+      | Some (Σ', μ', x, ext) with g _ x (weaken_env ext E) μ' :=
+          { | None := None;
+            | Some (_, μ'', y, ext') := Some (_, μ'', y, ext ⊚ ext') } }.
 
 Infix ">>=" := bind (at level 20, left associativity).
 
-Equations ret : ∀ {Γ A}, A → M Γ A :=
-  ret a γ := Some a.
+Definition transp_op {Γ Σ P} (x : Store Σ -> P Σ) : M Γ P Σ :=
+  fun E μ => Some (Σ, μ, x μ, refl_incl).
 
-Equations getEnv : ∀ {Γ}, M Γ (Env Γ) :=
-  getEnv γ := Some γ.
+Equations ret : ∀ {Γ Σ P}, P Σ → M Γ P Σ :=
+  ret (Σ:=Σ) a E μ := Some (Σ, μ, a, refl_incl).
 
-Equations usingEnv : ∀ {Γ Γ' A}, Env Γ → M Γ A → M Γ' A :=
-  usingEnv γ m γ' := m γ.
+Equations getEnv : ∀ {Γ Σ}, M Γ (Env Γ) Σ :=
+  getEnv (Σ:=Σ) E μ := Some (Σ, μ, E, refl_incl).
 
-Equations timeout : ∀ {Γ A}, M Γ A :=
-  timeout _ := None.
+Equations usingEnv {Γ Γ' Σ P} (E : Env Γ Σ) (m : M Γ P Σ) : M Γ' P Σ :=
+  usingEnv E m E' μ := m E μ.
 
-Equations eval : ∀ (n : nat) {Γ t} (e : Expr Γ t), M Γ (Val t) :=
-  eval 0 _             := timeout;
-  eval (S k) tt        := ret val_unit;
-  eval (S k) (var x)   := getEnv >>= fun E => ret (lookup E x);
-  eval (S k) (abs x)   := getEnv >>= fun E => ret (val_closure x E);
-  eval (S k) (app (Γ:=Γ) f arg) := eval k f >>= (#{ | val_closure e' E =>
-                                               eval k arg >>= fun a' => usingEnv (all_cons a' E) (eval k e')}).
+Equations timeout : ∀ {Γ Σ P}, M Γ P Σ :=
+  timeout _ _ := None.
+
+Section StoreOps.
+  Context {Σ : StoreTy} {Γ : Ctx} {t : Ty}.
+
+  Equations storeM (v : Val t Σ) : M Γ (Val (ref t)) Σ :=
+    storeM v E μ :=
+      let v : Val t (t :: Σ) := weaken_val store_ext_incl v in
+      let μ' := map_all (fun t' => weaken_val store_ext_incl) μ in
+      Some (t :: Σ, all_cons v μ', val_loc here, store_ext_incl).
+
+  Equations derefM (l : t ∈ Σ) : M Γ (Val t) Σ :=
+    derefM l := transp_op (lookup_store l).
+
+  Equations updateM (l : t ∈ Σ) (v : Val t Σ) : M Γ (Val unit) Σ :=
+    updateM l v E μ := Some (Σ, update_store l v μ, val_unit, refl_incl).
+End StoreOps.
+
+Reserved Notation "P ⊛ Q" (at level 10).
+
+Inductive storepred_prod (P Q : StoreTy -> Type) : StoreTy -> Type :=
+  | storepred_pair {Σ} : P Σ -> Q Σ -> (P ⊛ Q) Σ
+where "P ⊛ Q" := (storepred_prod P Q).
+Arguments storepred_pair {P Q Σ}.
+
+Class Weakenable (P : StoreTy -> Type) : Type :=
+  weaken : forall {Σ Σ'}, Σ ⊑ Σ' -> P Σ -> P Σ'.
+
+Instance val_weaken {t} : Weakenable (Val t).
+Proof. intros Σ Σ' incl. apply (weaken_val incl). Defined.
+
+Instance env_weaken {Γ} : Weakenable (Env Γ).
+Proof. intros Σ Σ' incl. apply (weaken_env incl). Defined.
+
+Instance loc_weaken (t : Ty) : Weakenable (In t).
+Proof. intros Σ Σ' incl. apply (pres_in incl). Defined.
+
+
+(* Equations strength {Σ Γ} {P Q : StoreTy -> Type} {w : Weakenable Q} (m : M Γ P Σ) (q : Q Σ) : M Γ (P ⊛ Q) Σ := *)
+(*   strength m q E μ := match m E μ with *)
+(*                       | None => None *)
+(*                       | Some (Σ, μ', p, ext) => Some (Σ, μ', storepred_pair p (weaken ext q), ext) *)
+(*                       end. *)
+
+Equations strength {Σ Γ} {P Q : StoreTy -> Type} {w : Weakenable Q} (m : M Γ P Σ) (q : Q Σ) : M Γ (P ⊛ Q) Σ :=
+  strength m q E μ with m E μ => {
+    | None => None;
+    | Some (Σ, μ', p, ext) => Some (Σ, μ', storepred_pair p (weaken ext q), ext) }.
+
+Infix "^" := strength.
+
+Equations(noind) eval (n : nat) {Γ Σ t} (e : Expr Γ t) : M Γ (Val t) Σ :=
+  eval 0 _                := timeout;
+  eval (S k) tt           := ret val_unit;
+  eval (S k) true         := ret val_true;
+  eval (S k) false        := ret val_false;
+  eval (S k) (ite b t f)  := eval k b >>= (#{ | _ | val_true => eval k t;
+                                              | _ | val_false => eval k f });
+
+  eval (S k) (var x)      := getEnv >>= fun Σ E => ret (lookup E x);
+  eval (S k) (abs x)      := getEnv >>= fun Σ E => ret (val_closure x E);
+  eval (S k) (app (Γ:=Γ) e1 e2) :=
+      eval k e1 >>= (#{ | _ | val_closure e' E =>
+                              (eval k e2 ^ E) >>= fun Σ' '(storepred_pair v E) =>
+                                                    usingEnv (all_cons v E) (eval k e')});
+  eval (S k) (new e)      := eval k e >>= fun Σ v => storeM v;
+  eval (S k) (deref l)    := eval k l >>= (#{ | _ | val_loc l => derefM l });
+  eval (S k) (assign l e) := eval k l >>= (#{ | _ | val_loc l =>
+                             (eval k e ^ l) >>= (#{ | _ | storepred_pair v l =>
+                                                          updateM l v >>= fun _ _ => ret val_unit }) }).
+
+Definition idu : Expr [] (unit ⇒ unit) :=
+  abs (var here).
+
+Definition idapp : Expr [] unit := app idu tt.
+
+Eval vm_compute in eval 100 idapp all_nil all_nil.
+
+Definition neg : Expr [] (bool ⇒ bool) :=
+  abs (ite (var here) false true).
+
+Definition letref {t u} (v : Expr [] t) (b : Expr [ref t] u) : Expr [] u :=
+  app (abs b) (new v).
+
+Equations weaken_expr {Γ Γ' t u} (e1 : Expr (Γ ++ Γ') t) : Expr (Γ ++ u :: Γ') t :=
+  weaken_expr tt             := tt;
+  weaken_expr true           := true;
+  weaken_expr false          := false;
+  weaken_expr (ite b t f)    := ite (weaken_expr b) (weaken_expr t) (weaken_expr f);
+  weaken_expr (var x)        := var _;
+  weaken_expr (abs (t:=t) x) := abs (weaken_expr (Γ := t :: Γ) x);
+  weaken_expr (app e1 e2)    := app (weaken_expr e1) (weaken_expr e2);
+  weaken_expr (new e)        := new (weaken_expr e);
+  weaken_expr (deref l)      := deref (weaken_expr l);
+  weaken_expr (assign l e)   := assign (weaken_expr l) (weaken_expr e).
+Next Obligation.
+  clear weaken_expr.
+  induction Γ in Γ', u, x |- *. now apply there. simpl.
+  depelim x. constructor. apply there. apply IHΓ. apply x.
+Defined.
+
+Definition seq {Γ u} (e1 : Expr Γ unit) (e2 : Expr Γ u) : Expr Γ u :=
+  app (abs (weaken_expr (Γ := []) e2)) e1.
+
+(* let x = ref true in
+   x := false; !x *)
+
+Definition letupdate : Expr [] bool :=
+  letref true (seq (assign (var here) false) (deref (var here))).
+
+Eval vm_compute in eval 100 letupdate all_nil all_nil.
+
+Extraction bind.
+
+
+
+
+
+
+
+
 
 Inductive eval_sem {Γ : Ctx} {env : Env Γ} : forall {t : Ty}, Expr Γ t -> Val t -> Prop :=
 | eval_tt (e : Expr Γ unit) : eval_sem e val_unit
